Foundation/Modal/Neighborhood/Logic/E.lean
@@ -33,7 +33,7 @@ instance : Hilbert.E ⪱ Hilbert.EK := by
       apply not_validOnFrameClass_of_exists_model_world;
       let M : Model := {
         World := Fin 3,
-        N := λ w =>
+        𝒩 := λ w =>
           match w with
           | 0 => {{0}, {0, 1, 2}}
           | 1 => ∅
@@ -67,7 +67,7 @@ instance : Hilbert.E ⪱ Hilbert.EN := by
       apply not_validOnFrameClass_of_exists_model_world;
       let M : Model := {
         World := Fin 1,
-        N := λ w => ∅,
+        𝒩 := λ w => ∅,
         Val := λ w => Set.univ
       };
       use M, 0;
