Foundation/Modal/Neighborhood/Logic/EC.lean
@@ -45,7 +45,7 @@ instance : Hilbert.E ⪱ Hilbert.EC := by
       apply not_validOnFrameClass_of_exists_model_world;
       let M : Model := {
         World := Fin 2,
-        N := λ w =>
+        𝒩 := λ w =>
           match w with
           | 0 => {{0}, {1}}
           | 1 => {∅},
